src/Narcissus/Examples/NetworkStack/UDP_Packet.v
@@ -73,19 +73,35 @@ Section UDP_Decoder.
   Definition UDP_encoder_impl r {sz} v :=
     Eval simpl in (projT1 UDP_encoder sz v 0 r tt).
 
-  Definition UDP_Packet_format_measure (udp_b : ByteString)
-    : nat :=
-    match (`(u, b') <- decode_unused_word' 16 udp_b;
-             `(u, b') <- decode_unused_word' 16 b';
-             decode_word' 16 b') with
-    | Some n => wordToNat (fst n)
-    | None => 0
-    end.
-
-  (* Step Two and a Half: Add some simple facts about correct packets
-   for the decoder automation. *)
+  Definition UDP_Packet_format_measure
+    : DecodeM (nat * ByteString) ByteString :=
+    fun t env =>
+      `(_, t', env') <- decode_word (sz := 16) t env;
+      `(_, t', env') <- decode_word (sz := 16) t' env';
+      decode_nat 16 t' env'.
 
   Lemma UDP_Packet_Header_Len_OK
+    : forall P P_inv,
+      cache_inv_Property P P_inv ->
+      CorrectDecoder monoid UDP_Packet_OK (constant True) (constant (constant True))
+    (format_word ◦ SourcePort ++
+     format_word ◦ DestPort ++ ((format_nat 16 ◦ Init.Nat.add 8) ◦ projT1 (P:=ByteBuffer.t)) ◦ Payload
+     ThenChecksum Pseudo_Checksum_Valid srcAddr destAddr udpLength (natToWord 8 17) OfSize 16
+     ThenCarryOn format_bytebuffer ◦ Payload) UDP_Packet_format_measure P
+    (fun (n : nat) (env : CacheFormat) =>
+     constant (forall (a : UDP_Packet) (t1 t2 : ByteString * CacheFormat),
+               word 16 ->
+               (format_word ◦ SourcePort ++
+                format_word ◦ DestPort ++ ((format_nat 16 ◦ Init.Nat.add 8) ◦ projT1 (P:=ByteBuffer.t)) ◦ Payload)
+                 a env t1 ->
+               (format_bytebuffer ◦ Payload) a (addE (snd t1) 16) t2 ->
+               bin_measure (fst t1) + 16 + bin_measure (fst t2) = n * 8)).
+  Proof.
+  Admitted.
+    (* Step Two and a Half: Add some simple facts about correct packets
+   for the decoder automation. *)
+
+  (*Lemma UDP_Packet_Header_Len_OK
     : forall (a : UDP_Packet) (ctx ctx' ctx'' : CacheFormat) (c : word 16) (b b'' ext : ByteString),
       (format_word ◦ SourcePort ++
         format_word ◦ DestPort ++ ((format_nat 16 ◦ Init.Nat.add 8) ◦ projT1 (P:=ByteBuffer.t)) ◦ Payload) a ctx ∋
@@ -131,7 +147,67 @@ Section UDP_Decoder.
     unfold UDP_Packet_OK in H1.
     revert H1; destruct (Payload a); simpl projT1.
     intros; omega.
-  Qed.
+  Qed. *)
+
+  (* Definition UDP_Packet_format_measure (udp_b : ByteString) *)
+  (*   : nat := *)
+  (*   match (`(u, b') <- decode_unused_word' 16 udp_b; *)
+  (*            `(u, b') <- decode_unused_word' 16 b'; *)
+  (*            decode_word' 16 b') with *)
+  (*   | Some n => wordToNat (fst n) *)
+  (*   | None => 0 *)
+  (*   end. *)
+
+  (* (* Step Two and a Half: Add some simple facts about correct packets *)
+  (*  for the decoder automation. *) *)
+
+  (* Lemma UDP_Packet_Header_Len_OK *)
+  (*   : forall (a : UDP_Packet) (ctx ctx' ctx'' : CacheFormat) (c : word 16) (b b'' ext : ByteString), *)
+  (*     (format_word ◦ SourcePort ++ *)
+  (*       format_word ◦ DestPort ++ ((format_nat 16 ◦ Init.Nat.add 8) ◦ projT1 (P:=ByteBuffer.t)) ◦ Payload) a ctx ∋ *)
+  (*      (b, ctx') -> *)
+  (*     (format_bytebuffer ◦ Payload) a ctx' ∋ (b'', ctx'') -> *)
+  (*     UDP_Packet_OK a -> *)
+  (*     (fun _ : UDP_Packet => 16 + (16 + 16)) a + (fun a' : UDP_Packet => 8 * projT1 (Payload a')) a + 16 = *)
+  (*     8 * UDP_Packet_format_measure *)
+  (*       (mappend *)
+  (*          (mappend b *)
+  (*                   (mappend (format_checksum ByteString AlignedByteString.ByteStringQueueMonoid ByteString_QueueMonoidOpt 16 c) b'')) ext). *)
+  (* Proof. *)
+  (*   intros; simpl. *)
+  (*   clear H0. *)
+  (*   pose proof mappend_assoc as H''; simpl in H''; *)
+  (*     rewrite <- !H''. *)
+  (*   unfold UDP_Packet_format_measure. *)
+  (*   unfold sequence_Format at 1 in H. *)
+  (*   eapply computes_to_compose_proj_decode_unused_word in H; *)
+  (*     let H' := fresh in *)
+  (*     destruct H as [? [? [? H'] ] ]; rewrite H'. *)
+  (*   unfold DecodeBindOpt; unfold BindOpt at 1; unfold If_Opt_Then_Else. *)
+  (*   unfold sequence_Format at 1 in H. *)
+  (*   eapply computes_to_compose_proj_decode_unused_word in H; *)
+  (*     let H' := fresh in *)
+  (*     destruct H as [? [? [? H'] ] ]; rewrite H'. *)
+  (*   unfold DecodeBindOpt; unfold BindOpt at 1; unfold If_Opt_Then_Else. *)
+  (*   eapply EquivFormat_Projection_Format in H. *)
+  (*   eapply EquivFormat_Projection_Format in H. *)
+  (*   eapply computes_to_proj_decode_nat in H; *)
+  (*     rewrite H. *)
+  (*   unfold fst. *)
+  (*   rewrite wordToNat_natToWord_idempotent; try reflexivity. *)
+  (*   rewrite !Plus.plus_assoc. *)
+  (*   clear; unfold Basics.compose; simpl. *)
+  (*   destruct (Payload a); simpl; omega. *)
+  (*   rewrite <- BinNat.N.compare_lt_iff. *)
+  (*   rewrite Nnat.N2Nat.inj_compare. *)
+  (*   rewrite Nnat.Nat2N.id. *)
+  (*   rewrite <- Compare_dec.nat_compare_lt. *)
+  (*   rewrite Npow2_nat. *)
+  (*   unfold Basics.compose. *)
+  (*   unfold UDP_Packet_OK in H1. *)
+  (*   revert H1; destruct (Payload a); simpl projT1. *)
+  (*   intros; omega. *)
+  (* Qed. *)
 
   Definition aligned_UDP_Packet_encoded_measure
              {sz} (ipv4_b : ByteBuffer.t sz)
@@ -164,20 +240,17 @@ Section UDP_Decoder.
   Ltac apply_new_combinator_rule ::=
     match goal with
     | H : cache_inv_Property ?mnd _
-      |- CorrectDecoder _ _ _ _ (?fmt1 ThenChecksum _ OfSize _ ThenCarryOn ?format2) _ _ _ =>
-      eapply compose_PseudoChecksum_format_correct;
+      |- CorrectDecoder _ _ _ _ (?fmt1 ThenChecksum _ OfSize _ ThenCarryOn ?format2) _ _ _ =>  eapply compose_PseudoChecksum_format_correct';
       [ repeat calculate_length_ByteString
       | repeat calculate_length_ByteString
       | exact H
       | solve_mod_8
       | solve_mod_8
-      | apply UDP_Packet_Header_Len_OK
+      |
       | intros; NormalizeFormats.normalize_format; apply_rules ]
   end.
 
-  Hint Extern 4 => intros; eapply (aligned_Pseudo_checksum_OK_1
-                                     _ _ _ _
-                                     (fun sz v => UDP_Packet_format_measure (build_aligned_ByteString v))).
+  Hint Extern 4 => eapply aligned_Pseudo_checksum_OK_1.
   Hint Extern 4 => eapply aligned_Pseudo_checksum_OK_2.
 
   (* Step Three: Synthesize a decoder and a proof that /it/ is correct. *)
@@ -185,7 +258,25 @@ Section UDP_Decoder.
     : CorrectAlignedDecoderFor UDP_Packet_OK UDP_Packet_Format.
   Proof.
     synthesize_aligned_decoder.
-  Defined.
+    intros.
+    simpl.
+    split.
+    instantiate (3 := format_word ◦ SourcePort ++
+                format_word ◦ DestPort ++ ((format_nat 16 ◦ Init.Nat.add 8) ◦ projT1 (P:=ByteBuffer.t)) ◦ Payload).
+    2: {
+      intros.
+      unfold sequence_Format at 1, ComposeOpt.compose, Bind2 in H1;
+        computes_to_inv; injections.
+      destruct v.
+      eexists _, _, _; split; eauto.
+      }
+    instantiate (2 := UDP_Packet_format_measure).
+    2: synthesize_cache_invariant.
+    admit.
+    unfold UDP_Packet_format_measure.
+    cbv beta; unfold decode_nat, sequence_Decode.
+    optimize_decoder_impl.
+  Admitted.
 
   (* Step Four: Extract the decoder function, and have /it/ start decoding
    at the start of the provided ByteString [v]. *)
